Examples/IHT_Splay_Tree.thy
@@ -131,7 +131,7 @@ lemma splay_code': "splay x (Tree.Node AB b CD) =
 declare splay_code' [rewrite]
 
 definition splay_time :: "'a::linorder \<Rightarrow> 'a tree \<Rightarrow> nat" where
-  "splay_time a t = 15 * t_splay a t"
+  "splay_time a t = 15 * T_splay a t"
 
 lemma splay_time_simp:
   "splay_time a Leaf = 15"
@@ -151,7 +151,7 @@ lemma splay_time_simp:
                else if rr = Leaf then 15 else splay_time a rr + 15))"
   by (auto split!: tree.split simp: splay_time_def)
 declare splay_time_simp [rewrite]
-setup \<open>add_fun_induct_rule (@{term_pat splay}, @{thm t_splay.induct[simplified LT EQ GT]})\<close>
+setup \<open>add_fun_induct_rule (@{term_pat splay}, @{thm T_splay.induct[simplified LT EQ GT]})\<close>
  
 
 lemma splay_not_Leaf: "splay x \<langle>l, a, r\<rangle> \<noteq> Leaf" by auto
@@ -204,10 +204,21 @@ definition insert_impl :: "'a::{heap,linorder} \<Rightarrow> 'a ptree \<Rightarr
           | GT \<Rightarrow> do {
               pp' := Node (lsub t') (val t') None;
               tree_constr_gen p' x (rsub t')
-            }})})"
+            }})})"                     
+
 
 definition insert_time :: "'a::linorder \<Rightarrow> 'a tree \<Rightarrow> nat" where [rewrite]:
-  "insert_time x t = splay_time x t + 4"
+  "insert_time x t = 15 * T_insert x t + 4"
+
+lemma insert_time_simps:
+  "insert_time a t = 15 + (if t = Leaf then 4 else splay_time a t + 4)"
+  by (auto split!: tree.split simp add: splay_time_def insert_time_def  T_insert_def)
+
+lemma aa2 [backward]:
+  assumes "True" (* TODO: fix this *)
+  shows 
+ "insert_time a t \<ge> (if t = Leaf then 4 else splay_time a t + 4)"
+  unfolding insert_time_simps by simp
 
 setup \<open>add_rewrite_rule @{thm Splay_Tree.insert.simps}\<close>
 setup \<open>fold add_rewrite_rule @{thms cmp_val.case}\<close>
@@ -218,6 +229,7 @@ lemma insert_correct [hoare_triple]:
     insert_impl x a
    <btree (insert x t)>\<^sub>t"
 @proof
+  @have "insert_time x t \<ge>\<^sub>t (if t = Leaf then 4 else splay_time x t + 4)"
   @case "t = Leaf"
   @let "V = cmp x (value (splay x t))"
   @cases V
@@ -242,7 +254,7 @@ partial_function (heap_time) splay_max_impl :: "'a::{heap,linorder} ptree \<Righ
                 rotate_ll p }}}})"
 
 definition splay_max_time :: "'a::linorder tree \<Rightarrow> nat" where
-  "splay_max_time t = 15 * t_splay_max t"
+  "splay_max_time t = 15 * T_splay_max t"
 
 lemma splay_max_time_simps [rewrite]:
   "splay_max_time Leaf = 15"
@@ -283,14 +295,24 @@ definition delete_impl :: "'a::{heap,linorder} \<Rightarrow> 'a ptree \<Rightarr
            else return p' }})"
 
 definition delete_time :: "'a::linorder \<Rightarrow> 'a tree \<Rightarrow> nat" where
-  "delete_time a t = 15 * t_delete a t + 5"
+  "delete_time a t = 15 * T_delete a t + 5"
 
-lemma delete_time_simps [rewrite]:
-  "delete_time a t = (if t = Leaf then 5 else splay_time a t + (case splay a t of
+lemma delete_time_simps:
+  "delete_time a t = 15 + (if t = Leaf then 5 else splay_time a t + (case splay a t of
     \<langle>l, x, r\<rangle> \<Rightarrow>
       if x=a then case l of Leaf \<Rightarrow> 5 | _ \<Rightarrow> splay_max_time l + 5
       else 5))"
-  by (auto split!: tree.split simp: splay_time_def splay_max_time_def delete_time_def t_delete_def)
+  by (auto split!: tree.split simp: splay_time_def splay_max_time_def delete_time_def T_delete_def)
+
+lemma aa [backward]:
+  assumes "True" (* TODO: fix this *)
+  shows 
+ "delete_time a t \<ge> (if t = Leaf then 5 else splay_time a t + (case splay a t of
+    \<langle>l, x, r\<rangle> \<Rightarrow>
+      if x=a then case l of Leaf \<Rightarrow> 5 | _ \<Rightarrow> splay_max_time l + 5
+      else 5))"
+  unfolding delete_time_simps by simp
+
 
 setup \<open>add_rewrite_rule @{thm Splay_Tree.delete_def}\<close>
 
@@ -299,6 +321,10 @@ lemma splay_delete_correct [hoare_triple]:
     delete_impl x a
    <btree (delete x t)>\<^sub>t"
 @proof
+  @have "delete_time x t \<ge>\<^sub>t (if t = Leaf then 5 else splay_time x t + (case splay x t of
+    \<langle>l, xx, r\<rangle> \<Rightarrow>
+      if xx=x then case l of Leaf \<Rightarrow> 5 | _ \<Rightarrow> splay_max_time l + 5
+      else 5))"
   @case "t = Leaf"
   @case "x = value (splay x t)"
 @qed
@@ -334,10 +360,10 @@ lemma a_splay [resolve]:
   assumes "bst t"
   shows "splay_time a t + splay_tree_P (splay a t) \<le> splay_tree_P t + splay_atime (size1 t)"
 proof -
-  have ineq1: "t_splay a t + nat (\<lceil>\<Phi> (splay a t)\<rceil>) \<le> nat (\<lceil>\<Phi> t\<rceil>) + nat (\<lceil>3 * log 2 (size1 t) + 1\<rceil> + 1)"
-    apply (rule amor_transfer [of "t_splay a t" "\<Phi>"])
-    apply (subst a_splay_def[symmetric])
-    using assms by (rule a_splay_ub3) (simp add: \<Phi>_nneg)+
+  have ineq1: "T_splay a t + nat (\<lceil>\<Phi> (splay a t)\<rceil>) \<le> nat (\<lceil>\<Phi> t\<rceil>) + nat (\<lceil>3 * log 2 (size1 t) + 1\<rceil> + 1)"
+    apply (rule amor_transfer [of "T_splay a t" "\<Phi>"])
+    apply (subst A_splay_def[symmetric])
+    using assms by (rule A_splay_ub3) (simp add: \<Phi>_nneg)+
   then show ?thesis
     by (simp only: splay_tree_P_def splay_atime_def splay_time_def)
 qed
@@ -362,20 +388,23 @@ lemma splay_atime_asym [asym_bound]:
   using abcd_lnx[of 30 15 3 0] by auto
 
 definition insert_atime :: "nat \<Rightarrow> nat" where
-  "insert_atime n = 15 * nat (\<lceil>4 * log 2 n + 2\<rceil> + 1) + 4"
+  "insert_atime n = 15 * nat (\<lceil>4 * log 2 n + 3\<rceil> + 1) + 4"
 
 lemma a_insert [backward]:
   assumes "bst t"
   shows "insert_time x t + splay_tree_P (insert x t) \<le> splay_tree_P t + insert_atime (size1 t)"
 proof -
-  have ineq1: "t_splay x t + nat \<lceil>\<Phi> (insert x t)\<rceil> \<le> nat \<lceil>\<Phi> t\<rceil> + nat (\<lceil>4 * \<phi> t + 2\<rceil> + 1)"
-    apply (rule amor_transfer [of "t_splay x t" "\<Phi>"])
+  have ineq1: "T_insert x t + nat \<lceil>\<Phi> (insert x t)\<rceil> \<le> nat \<lceil>\<Phi> t\<rceil> + nat (\<lceil>4 * \<phi> t + 3\<rceil> + 1)"
+    apply (rule amor_transfer [of "T_insert x t" "\<Phi>"])
     using assms by (rule amor_insert) (simp add: \<Phi>_nneg)+
   then show ?thesis
     by (simp only: insert_time_def splay_tree_P_def insert_atime_def splay_time_def)
 qed
 
-lemma insert_atime_alt: "\<forall>\<^sub>F x in sequentially. real (insert_atime x) = 49 + 15 * real (nat (\<lceil>4 * log 2 (real x)\<rceil>))"
+
+
+
+lemma insert_atime_alt: "\<forall>\<^sub>F x in sequentially. real (insert_atime x) = 64 + 15 * real (nat (\<lceil>4 * log 2 (real x)\<rceil>))"
   unfolding eventually_sequentially apply(rule exI[where x=1])  
   apply (auto simp: insert_atime_def) apply(subst nat_add_distrib)
   apply auto apply(rule less_le_trans[of _ 0] ) using log2_gt_zero by auto
@@ -383,7 +412,7 @@ lemma insert_atime_alt: "\<forall>\<^sub>F x in sequentially. real (insert_atime
 lemma insert_atime_asym [asym_bound]:
   "(\<lambda>n. insert_atime n) \<in> \<Theta>(\<lambda>x. ln (real x))"
   apply(rule landau_theta.ev_eq_trans2[OF insert_atime_alt]) 
-  using abcd_lnx[of 49 15 4 0] by auto
+  using abcd_lnx[of 64 15 4 0] by auto
 
 lemma splay_tree_insert_amor [hoare_triple]:
   "bst t \<Longrightarrow>
@@ -395,20 +424,20 @@ lemma splay_tree_insert_amor [hoare_triple]:
 @qed
 
 definition delete_atime :: "nat \<Rightarrow> nat" where
-  "delete_atime n = 15 * nat (\<lceil>6 * log 2 n + 2\<rceil> + 1) + 5"
+  "delete_atime n = 15 * nat (\<lceil>6 * log 2 n + 3\<rceil> + 1) + 5"
 
 lemma a_delete [backward]:
   assumes "bst t"
   shows "delete_time x t + splay_tree_P (delete x t) \<le> splay_tree_P t + delete_atime (size1 t)"
 proof -
-  have ineq1: "t_delete x t + nat \<lceil>\<Phi> (delete x t)\<rceil> \<le> nat \<lceil>\<Phi> t\<rceil> + nat (\<lceil>6 * \<phi> t + 2\<rceil> + 1)"
-    apply (rule amor_transfer [of "t_delete x t" "\<Phi>"])
+  have ineq1: "T_delete x t + nat \<lceil>\<Phi> (delete x t)\<rceil> \<le> nat \<lceil>\<Phi> t\<rceil> + nat (\<lceil>6 * \<phi> t + 3\<rceil> + 1)"
+    apply (rule amor_transfer [of "T_delete x t" "\<Phi>"])
     using assms by (rule amor_delete) (simp add: \<Phi>_nneg)+
   then show ?thesis
     by (simp only: delete_time_def splay_tree_P_def delete_atime_def)
 qed
 
-lemma delete_atime_alt: "\<forall>\<^sub>F x in sequentially. real (delete_atime x) = 50 + 15 * real (nat (\<lceil>6 * log 2 (real x)\<rceil>))"
+lemma delete_atime_alt: "\<forall>\<^sub>F x in sequentially. real (delete_atime x) = 65 + 15 * real (nat (\<lceil>6 * log 2 (real x)\<rceil>))"
   unfolding eventually_sequentially apply(rule exI[where x=1])  
   apply (auto simp: delete_atime_def) apply(subst nat_add_distrib)
   apply auto apply(rule less_le_trans[of _ 0] ) using log2_gt_zero by auto
@@ -416,7 +445,7 @@ lemma delete_atime_alt: "\<forall>\<^sub>F x in sequentially. real (delete_atime
 lemma delete_atime_asym [asym_bound]:
   "(\<lambda>n. delete_atime n) \<in> \<Theta>(\<lambda>x. ln (real x))" 
   apply(rule landau_theta.ev_eq_trans2[OF delete_atime_alt]) 
-  using abcd_lnx[of 50 15 6 0] by auto
+  using abcd_lnx[of 65 15 6 0] by auto
 
 lemma splay_tree_delete_amor [hoare_triple]:
   "bst t \<Longrightarrow>
@@ -451,24 +480,152 @@ lemma size1_set_tree [rewrite]:
   "bst t \<Longrightarrow> card (set_tree t) + 1 = size1 t"
   using size_set_tree by auto
 
-setup \<open>add_forward_prfstep_cond @{thm bst_splay} [with_term "splay ?a ?t"]\<close>
-setup \<open>add_rewrite_rule @{thm set_splay}\<close>
+(* some now commented-out proofs in Splay_Tree.Splay_Tree by Nipkow *)
+
+lemma ST_set_splay: "set_tree(Splay_Tree.splay a t) = set_tree t"
+proof(induction a t rule: splay.induct)
+  case (6 a)
+  with Splay_Tree.splay_not_Leaf[OF 6(3), of a] show ?case by(fastforce)
+next
+  case (8 _ a)
+  with Splay_Tree.splay_not_Leaf[OF 8(3), of a] show ?case by(fastforce)
+next
+  case (11 _ a)
+  with Splay_Tree.splay_not_Leaf[OF 11(3), of a] show ?case by(fastforce)
+next
+  case (14 _ a)
+  with Splay_Tree.splay_not_Leaf[OF 14(3), of a] show ?case by(fastforce)
+qed auto
+
+lemma ST_set_insert: "set_tree(insert a t) = Set.insert a (set_tree t)"
+  apply(cases t)
+ apply simp
+using ST_set_splay[of a t]
+  by(simp split: tree.split) fastforce
+
+lemma splay_max_Leaf: "splay_max t = Tree.Node l a r \<Longrightarrow> r = Leaf"
+by(induction t arbitrary: l rule: splay_max.induct)
+  (auto split: tree.splits if_splits)
+
+lemma splay_to_root: "\<lbrakk> bst t;  splay a t = t' \<rbrakk> \<Longrightarrow>
+  a \<in> set_tree t \<longleftrightarrow> (\<exists>l r. t' = Tree.Node l a r)"
+proof(induction a t arbitrary: t' rule: splay.induct)
+  case (6 a)
+  with Splay_Tree.splay_not_Leaf[OF 6(3), of a] show ?case by auto
+next
+  case (8 _ a)
+  with Splay_Tree.splay_not_Leaf[OF 8(3), of a] show ?case by auto
+next
+  case (11 _ a)
+  with Splay_Tree.splay_not_Leaf[OF 11(3), of a] show ?case by auto
+next
+  case (14 _ a)
+  with Splay_Tree.splay_not_Leaf[OF 14(3), of a] show ?case by auto
+qed fastforce+
+
+lemma set_splay_max: "set_tree(splay_max t) = set_tree t"
+apply(induction t rule: splay_max.induct)
+   apply(simp)
+  apply(simp)
+apply(force split: tree.split)
+done
+
+lemma ST_set_delete: assumes "bst t"
+shows "set_tree (Splay_Tree.delete a t) = set_tree t - {a}"
+proof(cases t)
+  case Leaf thus ?thesis by(simp add: delete_def)
+next
+  case (Node l x r)
+  obtain l' x' r' where sp[simp]: "splay a (Tree.Node l x r) = Tree.Node l' x' r'"
+    by (metis neq_Leaf_iff splay_Leaf_iff)
+  show ?thesis
+  proof cases
+    assume [simp]: "x' = a"
+    show ?thesis
+    proof cases
+      assume "l' = Leaf"
+      thus ?thesis
+        using Node assms ST_set_splay[of a "Tree.Node l x r"] bst_splay[of "Tree.Node l x r" a]
+        by(simp add: delete_def split: tree.split prod.split)(fastforce)
+    next
+      assume "l' \<noteq> Leaf"
+      moreover then obtain l'' m r'' where "splay_max l' = Tree.Node l'' m r''"
+        using splay_max_Leaf_iff tree.exhaust by blast
+      moreover have "a \<notin> set_tree l'"
+        by (metis (no_types) Node assms less_irrefl sp splay_bstL)
+      ultimately show ?thesis
+        using Node assms ST_set_splay[of a "Tree.Node l x r"] bst_splay[of "Tree.Node l x r" a]
+          splay_max_Leaf[of l' l'' m r''] set_splay_max[of l']
+        by(clarsimp simp: delete_def split: tree.split) auto
+    qed
+  next
+    assume "x' \<noteq> a"
+    thus ?thesis using Node assms ST_set_splay[of a "Tree.Node l x r"] splay_to_root[OF _ sp]
+      by (simp add: delete_def)
+  qed
+qed
+
+lemma bst_splay_max: "bst t \<Longrightarrow> bst (splay_max t)"
+proof(induction t rule: splay_max.induct)
+  case (3 l b rl c rr)
+  { fix rrl' d' rrr'
+    have "splay_max rr = Tree.Node rrl' d' rrr'
+       \<Longrightarrow> \<forall>x \<in> set_tree(Tree.Node rrl' d' rrr'). c < x" 
+      using "3.prems" set_splay_max[of rr]
+      by (clarsimp split: tree.split simp: ball_Un)
+  }
+  with 3 show ?case by (fastforce split: tree.split simp: ball_Un)
+qed auto
+
+lemma bst_delete: assumes "bst t" shows "bst (delete a t)"
+  proof(cases t)
+  case Leaf thus ?thesis by(simp add: delete_def)
+next
+  case (Node l x r)
+  obtain l' x' r' where sp[simp]: "splay a (Tree.Node l x r) = Tree.Node l' x' r'"
+    by (metis neq_Leaf_iff splay_Leaf_iff)
+  show ?thesis
+  proof cases
+    assume [simp]: "x' = a"
+    show ?thesis
+    proof cases
+      assume "l' = Leaf"
+      thus ?thesis using Node assms bst_splay[of "Tree.Node l x r" a]
+        by(simp add: delete_def split: tree.split prod.split)
+    next
+      assume "l' \<noteq> Leaf"
+      thus ?thesis
+        using Node assms ST_set_splay[of a "Tree.Node l x r"] bst_splay[of "Tree.Node l x r" a]
+          bst_splay_max[of l'] set_splay_max[of l']
+        by(clarsimp simp: delete_def split: tree.split)
+          (metis (no_types) insertI1 less_trans)
+    qed
+  next
+    assume "x' \<noteq> a"
+    thus ?thesis using Node assms bst_splay[of "Tree.Node l x r" a]
+      by(auto simp: delete_def split: tree.split prod.split)
+  qed
+qed
+
+
+setup \<open>add_forward_prfstep_cond @{thm bst_splay} [with_term "splay ?x ?t"]\<close>
+setup \<open>add_rewrite_rule @{thm ST_set_splay}\<close>
 
 lemma splay_tree_splay_rule [hoare_triple]:
   "<splay_tree_set S a * $(splay_atime (card S + 1))>
     splay_impl x a
    <splay_tree_set S>\<^sub>t" by auto2
 
-setup \<open>add_forward_prfstep_cond @{thm bst_insert} [with_term "insert ?a ?t"]\<close>
-setup \<open>add_rewrite_rule @{thm set_insert}\<close>
+setup \<open>add_forward_prfstep_cond @{thm bst_insert} [with_term "Splay_Tree.insert ?x ?t"]\<close>
+setup \<open>add_rewrite_rule @{thm ST_set_insert}\<close>
 
 lemma splay_tree_insert_rule [hoare_triple]:
   "<splay_tree_set S a * $(insert_atime (card S + 1))>
     insert_impl x a
    <splay_tree_set ({x} \<union> S)>\<^sub>t" by auto2
 
-setup \<open>add_forward_prfstep_cond @{thm bst_delete} [with_term "delete ?a ?t"]\<close>
-setup \<open>add_rewrite_rule @{thm set_delete}\<close>
+setup \<open>add_forward_prfstep_cond @{thm bst_delete} [with_term "Splay_Tree.delete ?a ?t"]\<close>
+setup \<open>add_rewrite_rule @{thm ST_set_delete}\<close>
 
 lemma splay_tree_delete_rule [hoare_triple]:
   "<splay_tree_set S a * $(delete_atime (card S + 1))>
